theories/Classes/Functions.v
@@ -20,22 +20,22 @@ Require Import Coq.Classes.Morphisms.
 Set Implicit Arguments.
 Unset Strict Implicit.
 
-Class Injective `(m : Morphism (A -> B) (RA ++> RB) f) : Prop :=
+Class Injective `(m : Proper (A -> B) (RA ++> RB) f) : Prop :=
   injective : forall x y : A, RB (f x) (f y) -> RA x y.
 
-Class Surjective `(m : Morphism (A -> B) (RA ++> RB) f) : Prop :=
+Class Surjective `(m : Proper (A -> B) (RA ++> RB) f) : Prop :=
   surjective : forall y, exists x : A, RB y (f x).
 
-Definition Bijective `(m : Morphism (A -> B) (RA ++> RB) (f : A -> B)) :=
+Definition Bijective `(m : Proper (A -> B) (RA ++> RB) (f : A -> B)) :=
   Injective m /\ Surjective m.
 
-Class MonoMorphism `(m : Morphism (A -> B) (eqA ++> eqB)) :=
+Class MonoMorphism `(m : Proper (A -> B) (eqA ++> eqB)) :=
   monic :> Injective m.
 
-Class EpiMorphism `(m : Morphism (A -> B) (eqA ++> eqB)) :=
+Class EpiMorphism `(m : Proper (A -> B) (eqA ++> eqB)) :=
   epic :> Surjective m.
 
-Class IsoMorphism `(m : Morphism (A -> B) (eqA ++> eqB)) :=
+Class IsoMorphism `(m : Proper (A -> B) (eqA ++> eqB)) :=
   { monomorphism :> MonoMorphism m ; epimorphism :> EpiMorphism m }.
 
-Class AutoMorphism `(m : Morphism (A -> A) (eqA ++> eqA)) {I : IsoMorphism m}.
+Class AutoMorphism `(m : Proper (A -> A) (eqA ++> eqA)) {I : IsoMorphism m}.
